src/fs/Examples.fs
@@ -2,358 +2,225 @@
 
 open GenOp
 
-let counterEx = 
-    <@@
-        let x = Array.zeroCreate 2
-        (not x.[0]) && (x.[1])
-    @@>
-
-/// <summary>
-/// Generate a ripple adder
-/// </summary>
-/// <param name="n">Number of bits for each input</param>
 let carryRippleAdder n =
-    <@@
-        fun (a : bool array) (b : bool array) ->
-        let result =  Array.zeroCreate (n)
-        result.[0] <- a.[0] <> b.[0]
-        let mutable carry = false
-        carry <- a.[0] <> b.[0]
-        result.[1] <- a.[1] <> b.[1] <> carry
-        allege (result.[1] = (a.[0] <> b.[0] <> a.[1] <> b.[1]))
-        for i in 2 .. n-1 do
-            carry <- (a.[i-1] && (b.[i-1] <> carry)) <> (carry && b.[i-1])
-            result.[i]  <-  a.[i] <> b.[i] <> carry
-        clean carry
-        result           
-    @@>
-(*
-let carryRippleAdder n =
-    <@@
-        let compute_carry (a : bool) (b : bool) (c : bool) =
-            (a && (b <> c)) <> (b && c)
-        in
-        fun (a : bool array) (b : bool array) (result : bool array) ->
-        result.[0] <- a.[0] <> b.[0]
-        let mutable carry = false
-        carry <- compute_carry a.[0] b.[0] carry
-        allege (carry = (a.[0] && b.[0]))
-        result.[1] <- a.[1] <> b.[1] <> carry
-        for i in 2 .. n-1 do
-            carry <- compute_carry a.[0] b.[0] carry
-            result.[i]  <-  a.[i] <> b.[i] <> carry
-            allege (result.[i] = (a.[i] <> b.[i] <> carry))
-        result           
-    @@>
-*)
-
-let mult22 n = 
-    <@@
-    let ctrlAddModn ctrl (a :bool array) (b :bool array) =
-        let mutable c = false
-        b.[0] <- b.[0] <> (a.[0]&&ctrl)
-        c <- c <> a.[0]
-        a.[0] <- a.[0] <> (c && b.[0])
-        b.[n-1] <- b.[n-1] <> (a.[n-1] && ctrl)
-        b.[n-1] <- b.[n-1] <> (a.[n-2] && ctrl)
-        a.[0] <- a.[0] <> (c && b.[0])
-        c <- c <> a.[0]
-        b.[0] <- b.[0] <> (c&&ctrl)
-        clean c
-    //let a =  Array.zeroCreate n
-    //let b =  Array.zeroCreate n
-    fun (a:bool array) (b:bool array) ->
-    let result = Array.zeroCreate (2*n)
-    for i in 0..n-1 do
-        ctrlAddModn a.[i] b result.[i..i+n-1]
-    result 
-    @@>
-
-let mult n = 
-    <@@
-    let ctrlAddModn ctrl (a :bool array) (b :bool array) =
-        let mutable c = false
-        b.[0] <- b.[0] <> (a.[0]&&ctrl)
-        c <- c <> a.[0]
-        a.[0] <- a.[0] <> (c && b.[0])
-        for i in 1 .. n - 2 do
-            b.[i] <- b.[i] <> (a.[i] && ctrl)
-            a.[i-1] <- a.[i-1] <> a.[i]
-            a.[i] <- a.[i] <> (a.[i-1] && b.[i])
-        b.[n-1] <- b.[n-1] <> (a.[n-1] && ctrl)
-        b.[n-1] <- b.[n-1] <> (a.[n-2] && ctrl)
-        for i in 2 .. n - 1 do
-            a.[n-i] <- a.[n-i] <> (a.[n-i-1] && b.[n-i])
-            a.[n-i-1] <- a.[n-i-1] <> a.[n-i]
-            b.[n-i] <- b.[n-i] <> (a.[n-i-1]&& ctrl)
-        a.[0] <- a.[0] <> (c && b.[0])
-        c <- c <> a.[0]
-        b.[0] <- b.[0] <> (c&&ctrl)
-        clean c
-    //let a =  Array.zeroCreate n
-    //let b =  Array.zeroCreate n
-    fun (a:bool array) (b:bool array) ->
-    let result = Array.zeroCreate (2*n)
-    for i in 0..n-1 do
-        ctrlAddModn a.[i] b result.[i..i+n-1]
-    result 
-    @@>
-
-let mult2 n = 
-    <@@
-    let addModn (a :bool array) (b :bool array) =
-        let mutable c = false
-        b.[0] <- b.[0] <> a.[0]
-        c <- c <> a.[0]
-        a.[0] <- a.[0] <> (c && b.[0])
-        for i in 1 .. n - 2 do
-            b.[i] <- b.[i] <> a.[i] 
-            a.[i-1] <- a.[i-1] <> a.[i]
-            a.[i] <- a.[i] <> (a.[i-1] && b.[i])
-        b.[n-1] <- b.[n-1] <> a.[n-1]
-        b.[n-1] <- b.[n-1] <> a.[n-2]
-        for i in 2 .. n - 1 do
-            a.[n-i] <- a.[n-i] <> (a.[n-i-1] && b.[n-i])
-            a.[n-i-1] <- a.[n-i-1] <> a.[n-i]
-            b.[n-i] <- b.[n-i] <> a.[n-i-1]
-        a.[0] <- a.[0] <> (c && b.[0])
-        c <- c <> a.[0]
-        b.[0] <- b.[0] <> c
-        clean c  
-    //let a =  Array.zeroCreate n
-    //let b =  Array.zeroCreate n
-    //let result = Array.zeroCreate (2*n)
-    fun (a:bool array) (b:bool array) ->
-    let result = Array.zeroCreate (2*n)
-    for i in 0..n-1 do
-        let addVal = 
-            if a.[i] then
-                b
-            else
-                Array.zeroCreate n
-        addModn addVal result.[i..i+n-1]
-    result 
-    @@>
-
-    (*
-let carryLookaheadAdder n = 
-    let adderSize = int (sqrt (float n))
-    let imSpacing = 2*(adderSize+1)
-    <@@
-        fun (a:bool array) (b:bool array) ->
-        let carryRipple (a:bool array) (b:bool array) (c:bool) (result: bool array) =
-            let mutable carry = c
-            result.[0] <- a.[0] <> b.[0] <> carry
-            for i in 1 .. adderSize - 1 do
-                carry <- (a.[i-1] && (carry <> b.[i-1])) <> (carry && b.[i-1])
-                result.[i]  <-  a.[i] <> b.[i] <> carry
-        let carryRippleC (a:bool array) (b:bool array) (c:bool) (result: bool array) =
-            let mutable carry = c
-            result.[0] <- a.[0] <> b.[0] <> carry
-            for i in 1 .. adderSize - 1 do
-                carry <- (a.[i-1] && (carry <> b.[i-1])) <> (carry && b.[i-1])
-                result.[i]  <-  a.[i] <> b.[i] <> carry
-            result.[adderSize] <- carry
-        let result = Array.zeroCreate (adderSize*adderSize)
-        let a0b0 = Array.zeroCreate (adderSize+1)
-        carryRipple a.[0..adderSize-1] b.[0..adderSize-1] false a0b0
-        carryRipple a.[0..adderSize-1] b.[0..adderSize-1] result.[0..adderSize-1] // a0b0
-        let a' = a.[adderSize .. adderSize*adderSize-1]
-        let b' = b.[adderSize .. adderSize*adderSize-1]
-        let intermediateResults = Array.zeroCreate (2*imSpacing*adderSize)
-        for i in 0 .. adderSize - 2 do
-            carryRippleFalse a'.[i*adderSize .. i*adderSize + adderSize-1] b'.[i*adderSize .. i*adderSize + adderSize-1] intermediateResults.[2*i*imSpacing..(2*i+1)*imSpacing - 1]
-            carryRippleTrue a'.[i*adderSize .. i*adderSize + adderSize-1] b'.[i*adderSize .. i*adderSize + adderSize-1] intermediateResults.[(2*i+1)*imSpacing..2*(i+1)*imSpacing]
-        let mutable carry = result.[adderSize]
-        for i in 0 .. adderSize - 2 do
-            for j in 0 .. adderSize - 1 do
-              result.[(i+1)*adderSize + j] <- (carry && intermediateResults.[i*imSpacing + j]) <> ((true <> carry) && intermediateResults.[i*imSpacing + adderSize + 1 + j])
-            carry <- (carry && intermediateResults.[i*imSpacing+adderSize]) <> ((true <> carry) && intermediateResults.[i*imSpacing+2*adderSize+1])
-        result
-      @@>*)
-
-let carryLookaheadAdder n = 
-    let adderSize = int (sqrt (float n))
-    let imSpacing = 2*(adderSize+1)
-    <@@
-        fun (a:bool array) (b:bool array) ->
-        let carryRipple (a:bool array) (b:bool array) (c:bool) (result: bool array) =
-            let mutable carry = c
-            result.[0] <- a.[0] <> b.[0] <> carry
-            for i in 1 .. adderSize - 1 do
-                carry <- (a.[i-1] && (carry <> b.[i-1])) <> (carry && b.[i-1])
-                result.[i]  <-  a.[i] <> b.[i] <> carry
-            result.[adderSize] <- carry
-        let result = Array.zeroCreate (adderSize*(adderSize-1))
-        let a0b0 = Array.zeroCreate (adderSize+1)
-        carryRipple a.[0..adderSize-1] b.[0..adderSize-1] false a0b0
-        let a' = a.[adderSize .. adderSize*adderSize-1]
-        let b' = b.[adderSize .. adderSize*adderSize-1]
-        let intermediateResults = Array.zeroCreate (2*adderSize*adderSize-2)
-        for i in 0 .. adderSize - 2 do
-            carryRipple a'.[i*adderSize .. i*adderSize + adderSize-1] b'.[i*adderSize .. i*adderSize + adderSize-1] false intermediateResults.[2*i*(adderSize+1)..(2*i+1)*(adderSize+1) - 1]
-            carryRipple a'.[i*adderSize .. i*adderSize + adderSize-1] b'.[i*adderSize .. i*adderSize + adderSize-1] true intermediateResults.[(2*i+1)*(adderSize+1)..2*(i+1)*(adderSize+1) - 1]
-        let mutable carry = a0b0.[adderSize]
-        for i in 0 .. adderSize - 2 do
-            for j in 0 .. adderSize - 1 do
-              result.[i*adderSize + j] <- (carry && intermediateResults.[i*imSpacing + j]) <> ((true <> carry) && intermediateResults.[i*imSpacing + adderSize + 1 + j])
-            carry <- (carry && intermediateResults.[i*imSpacing+adderSize]) <> ((true <> carry) && intermediateResults.[i*imSpacing+2*adderSize+1])
-        Array.concat [a0b0.[0..adderSize-1]; result]
-      @@>
-//
-//        //<- c.[i] || (for j in 0..i do ttt <- ttt && c.[j])
-////        for i in 1..n do 
-////            temp.[0] <- a.[i-1] && b.[i-1] 
-////            for j in 1..i-1 do 
-////                temp.[j] <- temp.[j] && (a.[]) // fix this 
-////            for j in 0..n-1 do 
-////                c.[i] <- c.[i] || temp.[j]
-////        
-////        for i in 0.. 
-//               
-//    @>
-
-/// <summary>
-/// Cuccaro adder 
-/// </summary>
-/// <param name="n">>Number of bits for each input</param>
-let addMod2 n =
     <@
-        fun (a:bool array) (b:bool array) ->
-        let mutable c = false
-        b.[0] <- b.[0] <> a.[0]
-        c <- c <> a.[0]
-        a.[0] <- a.[0] <> (c && b.[0])
-        a.[0] <- a.[0] <> (c && b.[0])
-        c <- c <> a.[0]
-        b.[0] <- b.[0] <> c
-        clean c
-        b          
+    fun (a : bool array) (b : bool array) (result : bool array) ->
+      let compute_carry (a : bool) (b : bool) (c : bool) =
+        (a && (b <> c)) <> (b && c) // a && b <> a && c <> b && c
+
+      let mutable carry = false
+      result.[0] <- a.[0] <> b.[0]
+      allege (carry = (a.[0] && b.[0]))
+      for i in 1 .. n-1 do
+        carry <- compute_carry a.[i-1] b.[i-1] carry
+        result.[i]  <-  a.[i] <> b.[i] <> carry
+        allege (result.[i] = (a.[i] <> b.[i] <> carry))
+      result           
     @>
 
 let addMod n =
     <@
-        fun (a:bool array) (b:bool array) ->
-        let mutable c = false
-        b.[0] <- b.[0] <> a.[0]
-        c <- c <> a.[0]
-        a.[0] <- a.[0] <> (c && b.[0])
-        for i in 1 .. n - 2 do
-            b.[i] <- b.[i] <> a.[i]
-            a.[i-1] <- a.[i-1] <> a.[i]
-            a.[i] <- a.[i] <> (a.[i-1] && b.[i])
-        b.[n-1] <- b.[n-1] <> a.[n-1]
-        b.[n-1] <- b.[n-1] <> a.[n-2]
-        for i in 2 .. n - 1 do
-            a.[n-i] <- a.[n-i] <> (a.[n-i-1] && b.[n-i])
-            a.[n-i-1] <- a.[n-i-1] <> a.[n-i]
-            b.[n-i] <- b.[n-i] <> a.[n-i-1]
-        a.[0] <- a.[0] <> (c && b.[0])
-        c <- c <> a.[0]
-        b.[0] <- b.[0] <> c
-        clean c
-        b          
+    fun (a:bool array) (b:bool array) ->
+      let mutable c = false
+      b.[0] <- b.[0] <> a.[0]
+      c <- c <> a.[0]
+      a.[0] <- a.[0] <> (c && b.[0])
+      for i in 1 .. n - 2 do
+        b.[i] <- b.[i] <> a.[i]
+        a.[i-1] <- a.[i-1] <> a.[i]
+        a.[i] <- a.[i] <> (a.[i-1] && b.[i])
+      b.[n-1] <- b.[n-1] <> a.[n-1]
+      b.[n-1] <- b.[n-1] <> a.[n-2]
+      for i in 2 .. n - 1 do
+        a.[n-i] <- a.[n-i] <> (a.[n-i-1] && b.[n-i])
+        a.[n-i-1] <- a.[n-i-1] <> a.[n-i]
+        b.[n-i] <- b.[n-i] <> a.[n-i-1]
+      a.[0] <- a.[0] <> (c && b.[0])
+      c <- c <> a.[0]
+      b.[0] <- b.[0] <> c
+      clean c
     @>
 
-let cucarro2 n =
-    <@@ 
-        fun (a:bool array) (b:bool array) ->
-        let mutable c = false
-        b.[0] <- b.[0] <> a.[0]
-        c <- c <> a.[0]
-        a.[0] <- a.[0] <> (c && b.[0])
-        b.[n-1] <- b.[n-1] <> a.[n-1]
-        b.[n-1] <- b.[n-1] <> a.[n-2]
-        a.[0] <- a.[0] <> (c && b.[0])
-        c <- c <> a.[0]
-        b.[0] <- b.[0] <> c
-        clean c
-        b
-    @@>
-
 let cucarro n =
-    <@@ 
-        fun (a:bool array) (b:bool array) ->
+    <@ 
+    fun (a:bool array) (b:bool array) ->
+      let mutable c = false
+      b.[0] <- b.[0] <> a.[0]
+      c <- c <> a.[0]
+      a.[0] <- a.[0] <> (c && b.[0])
+      for i in 1 .. n - 2 do
+        b.[i] <- b.[i] <> a.[i]
+        a.[i-1] <- a.[i-1] <> a.[i]
+        a.[i] <- a.[i] <> (a.[i-1] && b.[i])
+      b.[n-1] <- b.[n-1] <> a.[n-1]
+      b.[n-1] <- b.[n-1] <> a.[n-2]
+      a.[0] <- a.[0] <> (c && b.[0])
+      c <- c <> a.[0]
+      b.[0] <- b.[0] <> c
+      clean c
+      b
+    @>
+
+
+let mult n = 
+    <@
+    fun (a:bool array) (b:bool array) ->
+      let ctrlAddModn ctrl (a :bool array) (b :bool array) =
         let mutable c = false
-        b.[0] <- b.[0] <> a.[0]
+        b.[0] <- b.[0] <> (a.[0]&&ctrl)
         c <- c <> a.[0]
         a.[0] <- a.[0] <> (c && b.[0])
         for i in 1 .. n - 2 do
-            b.[i] <- b.[i] <> a.[i]
-            a.[i-1] <- a.[i-1] <> a.[i]
-            a.[i] <- a.[i] <> (a.[i-1] && b.[i])
-        b.[n-1] <- b.[n-1] <> a.[n-1]
-        b.[n-1] <- b.[n-1] <> a.[n-2]
+          b.[i] <- b.[i] <> (a.[i] && ctrl)
+          a.[i-1] <- a.[i-1] <> a.[i]
+          a.[i] <- a.[i] <> (a.[i-1] && b.[i])
+        b.[n-1] <- b.[n-1] <> (a.[n-1] && ctrl)
+        b.[n-1] <- b.[n-1] <> (a.[n-2] && ctrl)
+        for i in 2 .. n - 1 do
+          a.[n-i] <- a.[n-i] <> (a.[n-i-1] && b.[n-i])
+          a.[n-i-1] <- a.[n-i-1] <> a.[n-i]
+          b.[n-i] <- b.[n-i] <> (a.[n-i-1]&& ctrl)
         a.[0] <- a.[0] <> (c && b.[0])
         c <- c <> a.[0]
-        b.[0] <- b.[0] <> c
+        b.[0] <- b.[0] <> (c&&ctrl)
         clean c
-        b
-    @@>
+
+      let result = Array.zeroCreate (2*n)
+      for i in 0..n-1 do
+        ctrlAddModn a.[i] b result.[i..i+n-1]
+      result 
+    @>
+
+let mult2 n = 
+    <@
+    fun (a:bool array) (b:bool array) ->
+      let result = Array.zeroCreate (2*n)
+      let addMod = (%addMod n)
+      for i in 0..n-1 do
+        let addVal = if a.[i] then b else Array.zeroCreate n
+        addMod addVal result.[i..i+n-1]
+      result 
+    @>
+
+let carryLookaheadAdder n = 
+    let adderSize = int (sqrt (float n))
+    let imSpacing = 2*(adderSize+1)
+    <@
+    fun (a:bool array) (b:bool array) ->
+      let carryRipple (a:bool array) (b:bool array) (c:bool) (result: bool array) =
+        let mutable carry = c
+        result.[0] <- a.[0] <> b.[0] <> carry
+        for i in 1 .. adderSize - 1 do
+          carry <- (a.[i-1] && (carry <> b.[i-1])) <> (carry && b.[i-1])
+          result.[i]  <-  a.[i] <> b.[i] <> carry
+        result.[adderSize] <- carry
+
+      let result = Array.zeroCreate (adderSize*(adderSize-1))
+      let a0b0 = Array.zeroCreate (adderSize+1)
+      let a' = a.[adderSize .. adderSize*adderSize-1]
+      let b' = b.[adderSize .. adderSize*adderSize-1]
+      let intermediateResults = Array.zeroCreate (2*adderSize*adderSize-2)
+      let mutable carry = a0b0.[adderSize]
+      carryRipple a.[0..adderSize-1] b.[0..adderSize-1] false a0b0
+      for i in 0 .. adderSize - 2 do
+        carryRipple a'.[i*adderSize .. i*adderSize + adderSize-1] 
+                    b'.[i*adderSize .. i*adderSize + adderSize-1] 
+                    false 
+                    intermediateResults.[2*i*(adderSize+1)..(2*i+1)*(adderSize+1) - 1]
+        carryRipple a'.[i*adderSize .. i*adderSize + adderSize-1] 
+                    b'.[i*adderSize .. i*adderSize + adderSize-1] 
+                    true 
+                    intermediateResults.[(2*i+1)*(adderSize+1)..2*(i+1)*(adderSize+1) - 1]
+      for i in 0 .. adderSize - 2 do
+        for j in 0 .. adderSize - 1 do
+          result.[i*adderSize + j] <- (carry && intermediateResults.[i*imSpacing + j]) <> 
+                                      ((true <> carry) && intermediateResults.[i*imSpacing + adderSize + 1 + j])
+        carry <- (carry && intermediateResults.[i*imSpacing+adderSize]) <> 
+                 ((true <> carry) && intermediateResults.[i*imSpacing+2*adderSize+1])
+      Array.concat [a0b0.[0..adderSize-1]; result]
+    @>
 
 let ma4 =
-    <@@
+    <@
         fun (a:bool array) (b:bool array) (c:bool array) ->
         let ma4 (a :bool array)  (b :bool array)  (c :bool array) = 
             let t =  Array.zeroCreate 4
             for i in 0 .. 3 do
-                t.[i] <- (a.[i] && (b.[i] <> c.[i])) <> (b.[i] && c.[i])
+              t.[i] <- (a.[i] && (b.[i] <> c.[i])) <> (b.[i] && c.[i])
             t
         ma4 a b c
-    @@>
-/// <summary>
-/// Runs a number of rounds of SHA-2
-/// </summary>
-/// <param name="n">number of rounds</param>
-let exprSha n = 
-    <@
-    fun (k :bool array) (w :bool array) (x :bool array) ->
-    let addMod2_32 (a :bool array) (b :bool array) =
-        let mutable c = false
-        b.[0] <- b.[0] <> a.[0]
-        c <- c <> a.[0]
-        a.[0] <- a.[0] <> (c && b.[0])
-        for i in 1 .. 30 do
-            b.[i] <- b.[i] <> a.[i]
-            a.[i-1] <- a.[i-1] <> a.[i]
-            a.[i] <- a.[i] <> (a.[i-1] && b.[i])
-        b.[31] <- b.[31] <> a.[31]
-        b.[31] <- b.[31] <> a.[30]
-        for i in 2 .. 32 - 1 do
-            a.[32-i] <- a.[32-i] <> (a.[31-i] && b.[32-i])
-            a.[31-i] <- a.[31-i] <> a.[32-i]
-            b.[32-i] <- b.[32-i] <> a.[31-i]
-        a.[0] <- a.[0] <> (c && b.[0])
-        c <- c <> a.[0]
-        b.[0] <- b.[0] <> c
-        clean c
+    @>
+    
+let SHA2 n = 
+  <@
+  fun (k :bool array) (w :bool array) (x :bool array) ->
+    let addMod = (%addMod 32)
     let ch (e :bool array)  (f :bool array)  (g :bool array) = 
-        let t =  Array.zeroCreate 32
-        for i in 0 .. 31 do
-            t.[i] <- e.[i] && f.[i] && g.[i]
-        t
+      let t =  Array.zeroCreate 32
+      for i in 0 .. 31 do
+        t.[i] <- e.[i] && f.[i] && g.[i]
+      t
     let ma (a :bool array)  (b :bool array)  (c :bool array) = 
-        let t =  Array.zeroCreate 32
-        for i in 0 .. 31 do
-            t.[i] <- (a.[i] && (b.[i] <> c.[i])) <> (b.[i] && c.[i])
-        t
-    let s0 a =
-        let a2 = rot 2 a  
-        let a13 = rot 13 a
-        let a22 = rot 22 a
-        let t =  Array.zeroCreate 32
-        for i in 0 .. 31 do
-            t.[i] <- a2.[i] <> a13.[i] <> a22.[i]
-        t
-    let s1 a =
-        let a6 = rot 6 a 
-        let a11 = rot 11 a
-        let a25 = rot 25 a 
-        let mutable t =  Array.zeroCreate 32
-        for i in 0 .. 31 do
-            t.[i] <- a6.[i] <> a11.[i] <> a25.[i]
-        t
+      let t =  Array.zeroCreate 32
+      for i in 0 .. 31 do
+        t.[i] <- (a.[i] && (b.[i] <> c.[i])) <> (b.[i] && c.[i])
+      t
+    let s0 (a :bool array) =
+      let t =  Array.zeroCreate 32
+      let a2 = rot 2 a
+      let a13 = rot 13 a
+      let a22 = rot 22 a
+      for i in 0 .. 31 do
+        t.[i] <- a2.[i] <> a13.[i] <> a22.[i]
+      t
+    let s1 (a :bool array) =
+      let t =  Array.zeroCreate 32
+      let a6 = rot 6 a
+      let a11 = rot 11 a
+      let a25 = rot 25 a
+      for i in 0 .. 31 do
+        t.[i] <- a6.[i] <> a11.[i] <> a25.[i]
+      t
     let hsh (x :bool array) =
+      let a = x.[0..31]
+      let b = x.[32..63]
+      let c = x.[64..95]
+      let d = x.[96..127]
+      let e = x.[128..159]
+      let f = x.[160..191]
+      let g = x.[192..223]
+      let h = x.[224..255] 
+      addMod (ch e f g) h
+      addMod (s0 a) h
+      addMod w h
+      addMod k h
+      addMod h d
+      addMod (ma a b c) h
+      addMod (s1 e) h
+    for i in 0 .. n - 1 do
+      hsh (rot (32*i % 256) x)
+    x
+  @>
+
+let SHA2Efficient n = 
+  <@
+    fun (k :bool array) (w :bool array) (x :bool array) ->
+      let addMod = (%addMod 32)
+      let ch (e :bool array)  (f :bool array)  (g :bool array) (t :bool array) = 
+        for i in 0 .. 31 do
+          t.[i] <- t.[i] <> (e.[i] && f.[i] && g.[i])
+      let ma (a :bool array)  (b :bool array)  (c :bool array) (t: bool array) = 
+        for i in 0 .. 31 do
+          t.[i] <- t.[i] <> ((a.[i] && (b.[i] <> c.[i])) <> (b.[i] && c.[i]))
+      let s0 a (t :bool array) =
+        for i in 0 .. 31 do
+          t.[i] <- (rot 2 a).[i] <> (rot 13 a).[i] <> (rot 22 a).[i]
+      let s1 a (t :bool array) =
+        for i in 0 .. 31 do
+          t.[i] <- (rot 6 a).[i] <> (rot 11 a).[i] <> (rot 25 a).[i]
+
+      let hsh (x :bool array) =
+        let mutable anc = Array.zeroCreate 32
         let a = x.[0..31]
         let b = x.[32..63]
         let c = x.[64..95]
@@ -362,188 +229,96 @@ let exprSha n =
         let f = x.[160..191]
         let g = x.[192..223]
         let h = x.[224..255]
-        addMod2_32 (ch e f g) h
-        addMod2_32 (s0 a) h
-        addMod2_32 w h
-        addMod2_32 k h
-        addMod2_32 h d
-        addMod2_32 (ma a b c) h
-        addMod2_32 (s1 e) h
-    for i in 0 .. n - 1 do
+        s1 e anc
+        addMod anc h
+        s1 e anc
+
+        ch e f g anc
+        addMod anc h
+        ch e f g anc
+
+        addMod k h
+        addMod w h
+        addMod h d
+
+        ma a b c anc
+        addMod anc h
+        ma a b c anc
+
+        s0 a anc
+        addMod anc h
+        s0 a anc
+        clean anc
+        
+      for i in 0 .. n - 1 do
         hsh (rot (32*i % 256) x)
-    x
-    @>
-
-let exprShaEfficient = 
-  <@
-    fun (k :bool array) (w :bool array) (x :bool array) ->
-    let addMod2_32 (a :bool array) (b :bool array) =
-        let mutable c = false
-        b.[0] <- b.[0] <> a.[0]
-        c <- c <> a.[0]
-        a.[0] <- a.[0] <> (c && b.[0])
-        for i in 1 .. 30 do
-            b.[i] <- b.[i] <> a.[i]
-            a.[i-1] <- a.[i-1] <> a.[i]
-            a.[i] <- a.[i] <> (a.[i-1] && b.[i])
-        b.[31] <- b.[31] <> a.[31]
-        b.[31] <- b.[31] <> a.[30]
-        for i in 2 .. 31 do
-            a.[32-i] <- a.[32-i] <> (a.[32-i-1] && b.[32-i])
-            a.[32-i-1] <- a.[32-i-1] <> a.[32-i]
-            b.[32-i] <- b.[32-i] <> a.[32-i-1]
-        a.[0] <- a.[0] <> (c && b.[0])
-        c <- c <> a.[0]
-        b.[0] <- b.[0] <> c
-        clean c
-    let ch (e :bool array)  (f :bool array)  (g :bool array) (t :bool array) = 
-        for i in 0 .. 31 do
-          t.[i] <- t.[i] <> (e.[i] && f.[i] && g.[i])
-    let ma (a :bool array)  (b :bool array)  (c :bool array) (t: bool array) = 
-        for i in 0 .. 31 do
-          t.[i] <- t.[i] <> ((a.[i] && (b.[i] <> c.[i])) <> (b.[i] && c.[i]))
-    let s0 a (t :bool array) =
-        let a2 = rot 2 a  
-        let a13 = rot 13 a
-        let a22 = rot 22 a
-        for i in 0 .. 31 do
-          t.[i] <- t.[i] <> (a2.[i] <> a13.[i] <> a22.[i])
-    let s1 a (t :bool array) =
-        let a6 = rot 6 a 
-        let a11 = rot 11 a
-        let a25 = rot 25 a 
-        for i in 0 .. 31 do
-          t.[i] <- t.[i] <> (a6.[i] <> a11.[i] <> a25.[i])
-    let a = x.[0..31]
-    let b = x.[32..63]
-    let c = x.[64..95]
-    let d = x.[96..127]
-    let e = x.[128..159]
-    let f = x.[160..191]
-    let g = x.[192..223]
-    let h = x.[224..255]
-//    let k = [| false; false; false; true; true; false; false; true; true; true; true; true; false;
-//               true; false; false ;false; true; false; true; false; false; false; true; false; true;
-//               false; false; false; false; true; false |]
-    let mutable anc = Array.zeroCreate 32
-    s1 e anc
-    addMod2_32 anc h
-    s1 e anc
-
-    ch e f g anc
-    addMod2_32 anc h
-    ch e f g anc
-
-    addMod2_32 k h
-    addMod2_32 w h
-    addMod2_32 h d
-
-    ma a b c anc
-    addMod2_32 anc h
-    ma a b c anc
-
-    s0 a anc
-    addMod2_32 anc h
-    s0 a anc
-
-    x
+      x
   @>
 
 
-/// <summary>
-/// Runs a number of rounds of MD5
-/// </summary>
-/// <param name="n">number of rounds</param>
-let exprMD5 n = 
+let MD5 n = 
     let s = [| 7; 12; 17; 22;  7; 12; 17; 22;  7; 12; 17; 22;  7; 12; 17; 22; 
                5;  9; 14; 20;  5;  9; 14; 20;  5;  9; 14; 20;  5;  9; 14; 20; 
                4; 11; 16; 23;  4; 11; 16; 23;  4; 11; 16; 23;  4; 11; 16; 23;
                6; 10; 15; 21;  6; 10; 15; 21;  6; 10; 15; 21;  6; 10; 15; 21 |] 
     <@
-    fun (M :bool array) (K :bool array) (A :bool array) (B :bool array) 
-        (C :bool array) (D :bool array) ->
+    fun (M :bool array) (K :bool array) (X :bool array) ->
+      let addMod = (%addMod 32)
 
-    let addMod2_32 (a :bool array) (b :bool array) =
-        let mutable c = false
-        b.[0] <- b.[0] <> a.[0]
-        c <- c <> a.[0]
-        a.[0] <- a.[0] <> (c && b.[0])
-        for i in 1 .. 30 do
-            b.[i] <- b.[i] <> a.[i]
-            a.[i-1] <- a.[i-1] <> a.[i]
-            a.[i] <- a.[i] <> (a.[i-1] && b.[i])
-        b.[31] <- b.[31] <> a.[31]
-        b.[31] <- b.[31] <> a.[30]
-        for i in 2 .. n - 1 do
-            a.[32-i] <- a.[32-i] <> (a.[31-i] && b.[32-i])
-            a.[31-i] <- a.[31-i] <> a.[32-i]
-            b.[32-i] <- b.[32-i] <> a.[31-i]
-        a.[0] <- a.[0] <> (c && b.[0])
-        c <- c <> a.[0]
-        b.[0] <- b.[0] <> c
-        clean c
-
-    let F (B : bool array)  (C : bool array)  (D : bool array) = 
+      let F (B : bool array)  (C : bool array)  (D : bool array) = 
         let t =  Array.zeroCreate 32
         for i in 0 .. 31 do
-            t.[i] <- (B.[i] && C.[i]) || ((B.[i] <> false) && D.[i]) 
+          t.[i] <- (B.[i] && C.[i]) || ((B.[i] <> false) && D.[i]) 
         t
-    
-    let G (B : bool array)  (C : bool array)  (D : bool array) = 
+      let G (B : bool array)  (C : bool array)  (D : bool array) = 
         let t =  Array.zeroCreate 32
         for i in 0 .. 31 do
-            t.[i] <- (D.[i] && B.[i]) || ((D.[i] <> false) && C.[i]) 
+          t.[i] <- (D.[i] && B.[i]) || ((D.[i] <> false) && C.[i]) 
         t
-    
-    let H (B : bool array)  (C : bool array)  (D : bool array) = 
+      let H (B : bool array)  (C : bool array)  (D : bool array) = 
         let t =  Array.zeroCreate 32
         for i in 0 .. 31 do
-            t.[i] <- (B.[i] <> C.[i] <> D.[i])
+          t.[i] <- (B.[i] <> C.[i] <> D.[i])
         t
-    
-    let I (B : bool array)  (C : bool array)  (D : bool array) = 
+      let I (B : bool array)  (C : bool array)  (D : bool array) = 
         let t =  Array.zeroCreate 32
         for i in 0 .. 31 do
-            t.[i] <- (C.[i] <> (B.[i] || (D.[i] <> false)))
+          t.[i] <- (C.[i] <> (B.[i] || (D.[i] <> false)))
         t
-
-    for i in 0 .. 15 do
+        
+      for i in  0 .. 15 do
+        let X = rot (32*i % 128) X
         let mutable t = Array.zeroCreate 32
-        addMod2_32 A t
-        addMod2_32 (F B C D) t
-        addMod2_32 K t
-        addMod2_32 M.[32*i..32*i+31] t
-        addMod2_32 (rot s.[i] t) B
-        //let temp = D
-        //D <- C; C <- B; A <- temp        
-    for i in 16 .. 31 do
+        addMod X.[0..31] t
+        addMod (F X.[32..63] X.[64..95] X.[96..127]) t
+        addMod K t
+        addMod M.[32*i..32*i+31] t
+        addMod (rot s.[i] t) X.[32..63]
+      for i in 16 .. 31 do
+        let X = rot (32*i % 128) X
         let mutable t = Array.zeroCreate 32
-        addMod2_32 A t
-        addMod2_32 (G B C D) t
-        addMod2_32 K t
-        addMod2_32 M.[32*((5*i+1)%16)..32*((5*i+1)%16)+31] t
-        addMod2_32 (rot s.[i] t) B
-        //let temp = D
-        //D <- C; C <- B; A <- temp        
-    for i in 32 .. 47 do        
+        addMod X.[0..31] t
+        addMod (G X.[32..63] X.[64..95] X.[96..127]) t
+        addMod K t
+        addMod M.[32*((5*i+1)%16)..32*((5*i+1)%16)+31] t
+        addMod (rot s.[i] t) X.[32..63]
+      for i in 32 .. 47 do
+        let X = rot (32*i % 128) X
         let mutable t = Array.zeroCreate 32
-        addMod2_32 A t
-        addMod2_32 (H B C D) t
-        addMod2_32 K t
-        addMod2_32 M.[32*((3*i+5)%16)..32*((3*i+5)%16)+31] t
-        addMod2_32 (rot s.[i] t) B
-        //let temp = D
-        //D <- C; C <- B; A <- temp        
-    for i in 48 .. 63 do      
+        addMod X.[0..31] t
+        addMod (H X.[32..63] X.[64..95] X.[96..127]) t
+        addMod K t
+        addMod M.[32*((3*i+5)%16)..32*((3*i+5)%16)+31] t
+        addMod (rot s.[i] t) X.[32..63]
+      for i in 48 .. 63 do
+        let X = rot (32*i % 128) X
         let mutable t = Array.zeroCreate 32
-        addMod2_32 A t
-        addMod2_32 (I B C D) t
-        addMod2_32 K t
-        addMod2_32 M.[32*((7*i)%16)..32*((7*i)%16)+31] t
-        addMod2_32 (rot s.[i] t) B
-        //let temp = D
-        //D <- C; C <- B; A <- temp        
-    Array.concat [A; B; C; D]
+        addMod X.[0..31] t
+        addMod (I X.[32..63] X.[64..95] X.[96..127]) t
+        addMod K t
+        addMod M.[32*((7*i)%16)..32*((7*i)%16)+31] t
+        addMod (rot s.[i] t) X.[32..63]
+      X
     @>
 
 let keccakf l =
@@ -553,57 +328,59 @@ let keccakf l =
   let r = [| 0; 36; 3; 41; 18; 1; 44; 10; 45; 2; 62; 6; 43;
              15; 61; 28; 55; 25; 21; 56; 27; 20; 39; 8; 14 |]
   let ind x y z = 5*w*(x % 5) + w*(y % 5) + z
+
   <@
     fun (A :bool array) (RC :bool array) ->
+      let bxor (a: bool array) (b: bool array) =
+        for i in 0..w-1 do
+          a.[i] <- a.[i] <> b.[i]
 
-    let bxor (a: bool array) (b: bool array) =
-      for i in 0..w-1 do
-        a.[i] <- a.[i] <> b.[i]
+      let theta (a: bool array) =
+        let A = a
+        let C = Array.zeroCreate (5*w)   // temporary storage
+        let D = Array.zeroCreate (5*w)   // temporary storage
+        for x in 0..4 do          // C stage
+          for y in 0..4 do
+            bxor C.[w*x..w*x + w-1] A.[5*w*x + w*y..5*w*x + w*y + w-1]
+        for x in 0..4 do          // D stage
+          bxor D.[w*x..w*x + w-1] C.[w*((((x-1) % 5) + 5) % 5)..w*((((x-1) % 5) + 5) % 5) + w-1]
+          bxor D.[w*x..w*x + w-1] (rot (1 % w) C.[w*((x+1) % 5)..w*((x+1) % 5) + w-1])
+        for x in 0..4 do          // A stage
+          for y in 0..4 do
+            bxor A.[5*w*x + w*y..5*w*x + w*y + w-1] D.[w*x..w*x + w-1]
+        A
 
-    let theta (a: bool array) =
-      let A = a
-      let C = Array.zeroCreate (5*w)   // temporary storage
-      let D = Array.zeroCreate (5*w)   // temporary storage
-      for x in 0..4 do          // C stage
+      let rhopi (A: bool array) =
+        let B = Array.zeroCreate (5*5*w) // temporary storage
+        for x in 0..4 do          // Shuffle indices
+          for y in 0..4 do
+            bxor B.[5*w*y + w*((2*x + 3*y) % 5)..5*w*y + w*((2*x + 3*y) % 5) + w-1] 
+                 (rot (r.[(w*x + y) % 25] % w) A.[5*w*x + w*y..5*w*x + w*y + w-1])
+        B
+
+      let chi (A: bool array) =
+        let C = Array.zeroCreate (5*w)   // temporary storage
         for y in 0..4 do
-          bxor C.[w*x..w*x + w-1] A.[5*w*x + w*y..5*w*x + w*y + w-1]
-      for x in 0..4 do          // D stage
-        bxor D.[w*x..w*x + w-1] C.[w*((((x-1) % 5) + 5) % 5)..w*((((x-1) % 5) + 5) % 5) + w-1]
-        bxor D.[w*x..w*x + w-1] (rot (1 % w) C.[w*((x+1) % 5)..w*((x+1) % 5) + w-1])
-      for x in 0..4 do          // A stage
-        for y in 0..4 do
-          bxor A.[5*w*x + w*y..5*w*x + w*y + w-1] D.[w*x..w*x + w-1]
-      A
+          for x in 0..4 do
+            for z in 0..w-1 do
+              C.[w*x + z] <- 
+                C.[w*x + z] <> A.[5*w*x + w*y + z] <> A.[5*w*((x+2) % 5) + w*y + z]
+                            <> (A.[5*w*((x+1) % 5) + w*y + z] && A.[5*w*((x+2) % 5) + w*y + z])
+          for x in 0..4 do
+            for z in 0..w-1 do
+              A.[5*w*x + w*y + z] <- C.[w*x + z]
+          for x in 0..4 do     // uncompute C
+            for z in 0..w-1 do
+              C.[w*x + z] <- 
+                C.[w*x + z] <> A.[5*w*x + w*y + z] <> A.[5*w*((x+2) % 5) + w*y + z]
+                            <> (A.[5*w*((x+1) % 5) + w*y + z] && A.[5*w*((x+2) % 5) + w*y + z])
+        A
 
-    let rhopi (A: bool array) =
-      let B = Array.zeroCreate (5*5*w) // temporary storage
-      for x in 0..4 do          // Shuffle indices
-        for y in 0..4 do
-          bxor B.[5*w*y + w*((2*x + 3*y) % 5)..5*w*y + w*((2*x + 3*y) % 5) + w-1] 
-               (rot (r.[w*x + y] % w) A.[5*w*x + w*y..5*w*x + w*y + w-1])
-      B
+      let iota (A: bool array) = 
+        bxor A.[0..w-1] RC
+        A
 
-    let chi (A: bool array) =
-      let C = Array.zeroCreate (5*w)   // temporary storage
-      for y in 0..4 do
-        for x in 0..4 do
-          for z in 0..w-1 do
-            C.[w*x + z] <- C.[w*x + z] <> A.[5*w*x + w*y + z] <> A.[5*w*((x+2) % 5) + w*y + z]
-                                <> (A.[5*w*((x+1) % 5) + w*y + z] && A.[5*w*((x+2) % 5) + w*y + z])
-        for x in 0..4 do
-          for z in 0..w-1 do
-            A.[5*w*x + w*y + z] <- C.[w*x + z]
-        for x in 0..4 do     // uncompute C
-          for z in 0..w-1 do
-            C.[w*x + z] <- C.[w*x + z] <> A.[5*w*x + w*y + z] <> A.[5*w*((x+2) % 5) + w*y + z]
-                                <> (A.[5*w*((x+1) % 5) + w*y + z] && A.[5*w*((x+2) % 5) + w*y + z])
-      A
-
-    let iota (A: bool array) = 
-      bxor A.[0..w-1] RC
-      A
-
-    iota (chi (rhopi (theta A)))
+      iota (chi (rhopi (theta A)))
   @>
 
 let keccakfInPlace l =
@@ -630,11 +407,6 @@ let keccakfInPlace l =
         inverseBits.[64*xOff + z] <- true
       else 
         inverseBits.[64*xOff + z] <- false
-(*
-  printf "[|"
-  Array.iter (fun x -> printf "%A;" x) inverseBits
-  printf "|]"
-*)
   let inverseBits0 = [|
     false;false;false;true;true;false;true;true;true;false;false;false;false;true;false;true;false;
     false;true;true;false;true;true;true;false;false;false;false;true;false;true;false;false;true;
@@ -658,130 +430,75 @@ let keccakfInPlace l =
 
   <@
     fun (A :bool array) (RC :bool array) ->
+      let bxor (a: bool array) (b: bool array) =
+        for i in 0..w-1 do
+          a.[i] <- a.[i] <> b.[i]
 
-    let bxor (a: bool array) (b: bool array) =
-      for i in 0..w-1 do
-        a.[i] <- a.[i] <> b.[i]
-
-    let theta (a: bool array) =
-      let A = Array.zeroCreate (5*5*w) // Store the result
-      let C = Array.zeroCreate (5*w)   // temporary storage
-      let D = Array.zeroCreate (5*w)   // temporary storage
-      for x in 0..4 do          // Copy input
-        for y in 0..4 do
-          bxor A.[5*w*x + w*y..5*w*x + w*y + w-1] a.[5*w*x + w*y..5*w*x + w*y + w-1]
-      for x in 0..4 do          // C stage
-        for y in 0..4 do
-          bxor C.[w*x..w*x + w-1] A.[5*w*x + w*y..5*w*x + w*y + w-1]
-      for x in 0..4 do          // D stage
-        bxor D.[w*x..w*x + w-1] C.[w*((((x-1) % 5) + 5) % 5)..w*((((x-1) % 5) + 5) % 5) + w-1]
-        bxor D.[w*x..w*x + w-1] (rot (1 % w) C.[w*((x+1) % 5)..w*((x+1) % 5) + w-1])
-      for x in 0..4 do          // A stage
-        for y in 0..4 do
-          bxor A.[5*w*x + w*y..5*w*x + w*y + w-1] D.[w*x..w*x + w-1]
-      for x in 0..4 do          // Cleanup D
-        bxor D.[w*x..w*x + w-1] C.[w*((((x-1) % 5) + 5) % 5)..w*((((x-1) % 5) + 5) % 5) + w-1]
-        bxor D.[w*x..w*x + w-1] (rot (1 % w) C.[w*((x+1) % 5)..w*((x+1) % 5) + w-1])
-      for x in 0..4 do          // Cleanup C
-        for y in 0..4 do
-          bxor C.[w*x..w*x + w-1] a.[5*w*x + w*y..5*w*x + w*y + w-1]
-      for x in 0..4 do
-        for y in 0..w-1 do
-          clean D.[w*x + y]
-      // inverse theta
-      for x in 0..4 do          // C stage
-        for y in 0..4 do
-          bxor C.[w*x..w*x + w-1] A.[5*w*x + w*y..5*w*x + w*y + w-1]
-      for i in 0..w-1 do        // A stage
-        for xOff in 0..4 do
-          for x in 0..4 do
-            for y in 0..4 do
-              for z in 0..w-1 do
-                a.[5*w*x + w*y + z] <- 
-                  a.[5*w*x + w*y + z] <> C.[w*((((x-xOff) % 5) + 5) % 5) + ((z + i) % w)]
-//                  a.[5*w*x + w*y + z] <> (inverseBits.[64*xOff + i] && 
-//                                          C.[w*((((x-xOff) % 5) + 5) % 5) + ((z + i) % 64)])
-      for x in 0..4 do          // Cleanup
-        for z in 0..w-1 do
-          clean C.[w*x + z]
+      let theta (a: bool array) =
+        let A = Array.zeroCreate (5*5*w) // Store the result
+        for x in 0..4 do          // A stage
           for y in 0..4 do
-            clean a.[5*w*x + w*y + z]
-      A
+            for z in 0..w-1 do
+              A.[5*w*x + w*y + z] <- A.[5*w*x + w*y + z] <> a.[5*w*x + w*y + z]
+              for yp in 0..4 do
+                A.[5*w*x + w*y + z] <- A.[5*w*x + w*y + z] <> 
+                                       a.[5*w*((((x-1) % 5) + 5) % 5) + w*yp + z] <>
+                                       a.[5*w*((((x+1) % 5) + 5) % 5) + w*yp + ((((z-1) % w) + w) % w)]
+        // inverse theta
+        for i in 0..w-1 do        // A stage
+          for xOff in 0..4 do
+            for x in 0..4 do
+              for y in 0..4 do
+                for z in 0..w-1 do
+                  for yp in 0..4 do
+                    a.[5*w*x + w*y + z] <- 
+                      a.[5*w*x + w*y + z] <> A.[w*((((x-xOff) % 5) + 5) % 5) + ((z + i) % 64)]
+                      //(inverseBits.[64*xOff + i] && A.[w*((((x-xOff) % 5) + 5) % 5) + ((z + i) % 64)])
+        clean a
+        A
 
-    let thetaNoTemp (a: bool array) =
-      let A = Array.zeroCreate (5*5*w) // Store the result
-      for x in 0..4 do          // A stage
-        for y in 0..4 do
-          for z in 0..w-1 do
-            A.[5*w*x + w*y + z] <- A.[5*w*x + w*y + z] <> a.[5*w*x + w*y + z]
-            for yp in 0..4 do
-              A.[5*w*x + w*y + z] <- A.[5*w*x + w*y + z] <> 
-                                     a.[5*w*((((x-1) % 5) + 5) % 5) + w*yp + z] <>
-                                     a.[5*w*((((x+1) % 5) + 5) % 5) + w*yp + ((((z-1) % w) + w) % w)]
-      // inverse theta
-      for i in 0..w-1 do        // A stage
-        for xOff in 0..4 do
-          for x in 0..4 do
-            for y in 0..4 do
-              for z in 0..w-1 do
-                for yp in 0..4 do
-                  a.[5*w*x + w*y + z] <- 
-                    a.[5*w*x + w*y + z] <> A.[5*w*((((x-xOff) % 5) + 5) % 5) + w*y + ((z + i) % w)]
-//                  a.[5*w*x + w*y + z] <> (inverseBits.[64*xOff + i] && 
-//                                          C.[w*((((x-xOff) % 5) + 5) % 5) + ((z + i) % 64)])
-      for x in 0..4 do          // Cleanup
-        for z in 0..w-1 do
+      let rhopi (A: bool array) =
+        let B = Array.zeroCreate (5*5*w) // temporary storage
+        for x in 0..4 do          // Shuffle indices
           for y in 0..4 do
-            clean a.[5*w*x + w*y + z]
-      A
+            bxor B.[5*w*y + w*((2*x + 3*y) % 5)..5*w*y + w*((2*x + 3*y) % 5) + w-1] 
+                 (rot (r.[(w*x + y) % 25] % w) A.[5*w*x + w*y..5*w*x + w*y + w-1])
+        for x in 0..4 do          // Uncompute A
+          for y in 0..4 do
+            bxor (rot (r.[w*x + y] % w) A.[5*w*x + w*y..5*w*x + w*y + w-1])
+                 B.[5*w*y + w*((2*x + 3*y) % 5)..5*w*y + w*((2*x + 3*y) % 5) + w-1] 
+        clean A
+        B
+      
+      let chi (B: bool array) =
+        let A = Array.zeroCreate (5*5*w) // Store the result
+        for x in 0..4 do         // Compute result
+          for y in 0..4 do
+            for z in 0..w-1 do
+              A.[5*w*x + y*w + z] <- A.[5*w*x + y*w + z] 
+                <> B.[5*w*x + y*w + z] <> B.[5*w*((x+2) % 5) + w*y + z]
+                <> (B.[5*w*((x+1) % 5) + w*y + z] && B.[5*w*((x+2) % 5) + w*y + z])
+        // inverse Chi
+        for x in 0..4 do          // Copy output onto B
+          for y in 0..4 do
+            bxor B.[5*w*x + w*y..5*w*x + w*y + w-1] A.[5*w*x + w*y..5*w*x + w*y + w-1]
+        for y in 0..4 do         // Uncompute B
+          for x in 0..5 do
+            for z in 0..w-1 do
+              B.[5*w*((3*x) % 5) + w*y + z] <- B.[5*w*((3*x) % 5) + w*y + z]
+                <> A.[5*w*((3*x) % 5) + w*y + z] <> B.[5*w*((3*x + 2) % 5) + w*y + z]
+                <> (B.[5*w*((3*x + 2) % 5) + w*y + z] && A.[5*w*((3*x + 1) % 5) + w*y + z])
+        clean B
+        A
+      
+      let iota (A: bool array) = 
+        bxor A.[0..w-1] RC
+        A
 
-    let rhopi (A: bool array) =
-      let B = Array.zeroCreate (5*5*w) // temporary storage
-      for x in 0..4 do          // Shuffle indices
-        for y in 0..4 do
-          bxor B.[5*w*y + w*((2*x + 3*y) % 5)..5*w*y + w*((2*x + 3*y) % 5) + w-1] 
-               (rot (r.[w*x + y] % w) A.[5*w*x + w*y..5*w*x + w*y + w-1])
-      for x in 0..4 do          // Uncompute A
-        for y in 0..4 do
-          bxor (rot (r.[w*x + y] % w) A.[5*w*x + w*y..5*w*x + w*y + w-1])
-               B.[5*w*y + w*((2*x + 3*y) % 5)..5*w*y + w*((2*x + 3*y) % 5) + w-1] 
-      for x in 0..4 do
-        for y in 0..4 do
-          for z in 0..w-1 do
-            clean A.[5*w*x + w*y + z]
-      B
-
-    let chi (B: bool array) =
-      let A = Array.zeroCreate (5*5*w) // Store the result
-      for x in 0..4 do         // Compute result
-        for y in 0..4 do
-          for z in 0..w-1 do
-            A.[5*w*x + y*w + z] <- A.[5*w*x + y*w + z] 
-              <> B.[5*w*x + y*w + z] <> B.[5*w*((x+2) % 5) + w*y + z]
-              <> (B.[5*w*((x+1) % 5) + w*y + z] && B.[5*w*((x+2) % 5) + w*y + z])
-      // inverse Chi
-      for x in 0..4 do          // Copy output onto B
-        for y in 0..4 do
-          bxor B.[5*w*x + w*y..5*w*x + w*y + w-1] A.[5*w*x + w*y..5*w*x + w*y + w-1]
-      for y in 0..4 do         // Uncompute B
-        for x in 0..5 do
-          for z in 0..w-1 do
-            B.[5*w*((3*x) % 5) + w*y + z] <- B.[5*w*((3*x) % 5) + w*y + z]
-              <> A.[5*w*((3*x) % 5) + w*y + z] <> B.[5*w*((3*x + 2) % 5) + w*y + z]
-              <> (B.[5*w*((3*x + 2) % 5) + w*y + z] && A.[5*w*((3*x + 1) % 5) + w*y + z])
-      for x in 0..4 do
-        for y in 0..4 do
-          for z in 0..w-1 do
-            clean B.[5*w*x + w*y + z]
-      A
-
-    let iota (A: bool array) = 
-      bxor A.[0..w-1] RC
-      A
-
-    iota (chi (rhopi (thetaNoTemp A)))
+      iota (chi (rhopi (theta A)))
   @>
 
+(*
 let chifun l = 
   let w = 1<<<l
   <@
@@ -898,40 +615,4 @@ let inversePositionsWt l =
   for x in 0..4 do
     printf "%d\n" inversePositions.[x]
   printf "Total: %d\n" total
-
-//Some examples used in the paper
-let circ1 =    
-    <@
-    let f a b = a || b
-    let g a b = a && b
-    let h a b c d = f a b <> g c d
-    h false false false false
-    @>
-
-let circ2  =
-    <@
-    let a = false
-    let mutable b = false
-    let c = (a&&b)
-    b <- b <> c
-    b
-    @>
-
-let circ3 = 
-    <@
-    let xor4 (a:bool array) (b:bool array) =
-        let c = Array.zeroCreate 4
-        for i in 0 .. 3 do
-            c.[i] <- a.[i] <> b.[i]
-        c
-    let and4 (a:bool array) (b:bool array) =
-        let d = Array.zeroCreate 4
-        for i in 0 .. 3 do
-            d.[i] <- a.[i] && b.[i]
-        d
-    let mutable a = Array.zeroCreate 4
-    let b = Array.zeroCreate 4
-    let c = Array.zeroCreate 4
-    a <- xor4 a b
-    and4 a c
-@>
+*)
