src/fs/Program.fs
@@ -15,115 +15,95 @@ open Interpreter
 open Examples
 open Equiv
 
-let runDirect program cleanupStrategy = 
-    let (top, gexp) = parseAST program
-    printf "gExp:\n%s\n" (show gexp);
-    let (top', eqs, bnds, typ) = inferTypes top [] gexp
-    let eqs =
-      let f c = match c with
-        | TCons (x, y) -> not (x = y)
-        | ICons (x, y) -> not (x = y)
-      List.filter f eqs
-//    printf "gExp:\n%s\n" (show gexp);
-//    printf "Equality constraints:\n%A\n" eqs;
-//    printf "Ordered constraints:\n%A\n" bnds;
-    let res = unify_eq top'  eqs bnds []
-    match res with
-      | None -> printf "Error: could not infer types\n"
-      | Some subs -> 
-          let gexp' = applySubs subs gexp
-          printf "Annotated gExp:\n%s\n" (show gexp');
-          let res = compileCirc (gexp', circInit)
-          let ver = compileBDD (gexp', bddInit)
-          match res with
-            | Err s -> printf "%s\n" s
-            | Val (_, circ) -> printf "Circuit:\n%s\n" (String.concat "\n" (prettyPrintCircuit circ));
-                               printf "Bits used: %d\n" (Set.count (uses circ));
-                               printf "Gates: %d\n" (List.length circ);
-                               printf "Toffolis: %d\n" (List.length (List.filter (fun x -> match x with RTOFF _ -> true | _ -> false) circ))
+type mode = 
+  | Default
+  | SpaceSave
 
-let runBool program cleanupStrategy = 
-    let (top, gexp) = parseAST program
-    let (top', eqs, bnds, typ) = inferTypes top [] gexp
-    let eqs =
-      let f c = match c with
-        | TCons (x, y) -> not (x = y)
-        | ICons (x, y) -> not (x = y)
-      List.filter f eqs
-    let res = unify_eq top'  eqs bnds []
-//    printf "gExp:\n%s\n" (show gexp);
-//    printf "Equality constraints:\n%A\n" eqs;
-//    printf "Ordered constraints:\n%A\n" bnds;
-    match res with
-      | None -> printf "Error: could not infer types\n"
-      | Some subs -> 
-          let gexp' = applySubs subs gexp
-          printf "Annotated gExp:\n%s\n" (show gexp');
-          let res = compile (gexp', bexpInit) cleanupStrategy
-          match res with
-            | Err s -> printf "%s\n" s
-            | Val (_, circ) -> printf "Circuit:\n%s\n" (String.concat "\n" (prettyPrintCircuit circ))
-                               printf "Bits used: %d\n" (Set.count (uses circ));
-                               printf "Gates: %d\n" (List.length circ);
-                               printf "Toffolis: %d\n" (List.length (List.filter (fun x -> match x with RTOFF _ -> true | _ -> false) circ))
+let info = true
+let verify = false
 
+let isToff = function
+  | RTOFF _ -> true
+  | _       -> false
+
+let run program mode cleanupStrategy = 
+  // Parsing
+  let (top, gexp) = parseAST program
+  if info then printf "gExp:\n%s\n" (show gexp)
+  // Type inference
+  let (top', eqs, bnds, typ) = inferTypes top [] gexp
+  let eqs =
+    let f c = match c with
+      | TCons (x, y) -> not (x = y)
+      | ICons (x, y) -> not (x = y)
+    List.filter f eqs
+  let res = unify_eq top' eqs bnds []
+  match res with
+    | None -> printf "Error: could not infer types\n"
+              printf "Equality constraints:\n%A\n" eqs
+              printf "Ordered constraints:\n%A\n" bnds
+    | Some subs -> 
+        let gexp' = applySubs subs gexp
+        if info then printf "Annotated gExp:\n%s\n" (show gexp');
+        // Verification
+        if verify then ignore <| compileBDD (gexp', bddInit)
+        // Compilation
+        let res = match mode with 
+          | Default   -> compileCirc (gexp', circInit)
+          | SpaceSave -> compile     (gexp', bexpInit) cleanupStrategy
+        match res with
+          | Err s -> printf "%s\n" s
+          | Val (_, circ) -> 
+              if info then 
+                printf "Bits used: %d\n" (Set.count (uses circ))
+                printf "Gates: %d\n" (List.length circ)
+                printf "Toffolis: %d\n" (List.length (List.filter isToff circ))
+              printf "%s" (printQCV circ (Set.count (uses circ)))
 
 [<EntryPoint>]
 let __main _ = 
-  printf "Carry-Ripple 8:\n"
-  ignore <| runDirect (carryRippleAdder 8) Pebbled
-  Console.Out.Flush()
   (*
-  printf "\nSHA (2 rounds):\n"
-  ignore <| runDirect (exprSha 2) Pebbled
-  Console.Out.Flush()
   printf "Carry-Ripple 32:\n"
-  ignore <| runDirect (carryRippleAdder 32) Pebbled
+  ignore <| run (carryRippleAdder 32) Default Pebbled
   Console.Out.Flush()
-  printf "\nCarry-Ripple 64:\n"
-  //ignore <| runDirect (carryRippleAdder 64) Pebbled
-  Console.Out.Flush()
-  printf "\nMult 32:\n"
-  //ignore <| runDirect (mult 32) Pebbled
-  Console.Out.Flush()
-  printf "\nMult 64:\n"
-  //ignore <| runDirect (mult 64) Pebbled
-  Console.Out.Flush()
-  (*
-  printf "\nCarry-Lookahead 32:\n"
-  ignore <| runDirect (carryLookaheadAdder 32) Pebbled
-  Console.Out.Flush()
-  printf "\nCarry-Lookahead 64:\n"
-  ignore <| runDirect (carryLookaheadAdder 64) Pebbled
-  Console.Out.Flush()*)
+
   printf "\nModular adder 32:\n"
-  ignore <| runDirect (addMod 32) Pebbled
+  ignore <| run (addMod 32) Default Pebbled
   Console.Out.Flush()
-  printf "\nModular adder 64:\n"
-  ignore <| runDirect (addMod 64) Pebbled
-  Console.Out.Flush()
+
   printf "\nCucarro adder 32:\n"
-  ignore <| runDirect (cucarro 32) Pebbled
+  ignore <| run (cucarro 32) Default Pebbled
   Console.Out.Flush()
-  printf "\nCucarro adder 64:\n"
-  ignore <| runDirect (cucarro 64) Pebbled
+
+  printf "\nMult 32:\n"
+  ignore <| run (mult 32) Default Pebbled
   Console.Out.Flush()
+
+  printf "\nCarry-Lookahead 32:\n"
+  ignore <| run (carryLookaheadAdder 32) Default Pebbled
+  Console.Out.Flush()
+
   printf "\nma4:\n"
-  ignore <| runDirect (ma4) Pebbled
+  ignore <| run (ma4) Default Pebbled
   Console.Out.Flush()
-  printf "\nSHA (2 rounds):\n"
-  ignore <| runDirect (exprSha 2) Pebbled
+
+  printf "\nSHA (64 rounds):\n"
+  ignore <| run (SHA2 2) Default Pebbled
   Console.Out.Flush()
-  printf "\nMD5 (2 rounds):\n"
-  ignore <| runDirect (exprMD5 2) Pebbled
+
+  printf "\nSHA (64 rounds) -- manual cleanup:\n"
+  ignore <| run (SHA2Efficient 2) Default Pebbled
   Console.Out.Flush()
-  printf "\nSHA (4 rounds):\n"
-  ignore <| runDirect (exprSha 4) Pebbled
+
+  printf "\nMD5 (64 rounds):\n"
+  ignore <| run (MD5 2) Default Pebbled
   Console.Out.Flush()
-  printf "\nSHA (8 rounds):\n"
-  ignore <| runDirect (exprSha 8) Pebbled
+*)
+  printf "\nKeccak (64 bit lanes):\n"
+  ignore <| run (keccakf 4) Default Pebbled
   Console.Out.Flush()
-  printf "\nSHA (16 rounds):\n"
-  ignore <| runDirect (exprSha 16) Pebbled
-  Console.Out.Flush()*)
+
+  printf "\nKeccak (64 bit lanes) -- in place:\n"
+  ignore <| run (keccakfInPlace 4) Default Pebbled
+  Console.Out.Flush()
   0
